SoftwareFoundations/ProgrammingLanguageFoundations/Equiv.lean
@@ -1,0 +1,256 @@
+/-
+# Program Equivalence
+-/
+
+import Mathlib.tactic.linarith
+
+import «SoftwareFoundations».«LogicalFoundations».«Maps»
+import «SoftwareFoundations».«LogicalFoundations».«Imp»
+
+/-
+## Behavioral Equivalence
+-/
+
+/-
+### Definitions
+-/
+
+def Arith.equiv (a₁ a₂: Arith): Prop := ∀ s: State, a₁.eval s = a₂.eval s
+def Logic.equiv (l₁ l₂: Logic): Prop := ∀ s: State, l₁.eval s = l₂.eval s
+
+example: (Arith.minus "X" "X").equiv (Arith.num 0) := by
+  unfold Arith.equiv
+  intro s
+  simp
+
+example: (Logic.eq (.minus "X" "X") 0).equiv .true := by
+  unfold Logic.equiv
+  intro s
+  simp
+  unfold Arith.eval
+  rfl
+
+def Command.equiv (c₁ c₂: Command): Prop := ∀ s₁ s₂: State, CommandEval c₁ s₁ s₂ ↔ CommandEval c₂ s₁ s₂
+def Command.refines (c₁ c₂: Command): Prop := ∀ s₁ s₂: State, CommandEval c₁ s₁ s₂ → CommandEval c₂ s₁ s₂
+
+/-
+### Simple Examples
+-/
+
+example (c: Command): (Command.seq .skip c).equiv c :=
+  fun s₁ s₂ =>
+    have mp: CommandEval (Command.seq .skip c) s₁ s₂ → CommandEval c s₁ s₂
+      | .seq .skip c _ _ s₃ (.skip s) h₂ => h₂
+    have mpr: CommandEval c s₁ s₂ → CommandEval (Command.seq .skip c) s₁ s₂
+      | .skip _                        => .seq _ _ _ _ _ (.skip _) (.skip _)
+      | .assign _ _ _ _ h              => .seq _ _ _ _ _ (.skip _) (.assign _ _ _ _ h)
+      | .seq _ _ _ s₂ _ h₁ h₂          => .seq _ _ _ _ _ (.skip _) (.seq _ _ _ s₂ _ h₁ h₂)
+      | .ifTrue _ _ _ _ _ h₁ h₂        => .seq _ _ _ _ _ (.skip _) (.ifTrue _ _ _ _ _ h₁ h₂)
+      | .ifFalse _ _ _ _ _ h₁ h₂       => .seq _ _ _ _ _ (.skip _) (.ifFalse _ _ _ _ _ h₁ h₂)
+      | .whileTrue _ s₂ _ _ _ h₁ h₂ h₃ => .seq _ _ _ _ _ (.skip _) (.whileTrue _ s₂ _ _ _ h₁ h₂ h₃)
+      | .whileFalse _ _ _ h₁           => .seq _ _ _ _ _ (.skip _) (.whileFalse _ _ _ h₁)
+    ⟨mp, mpr⟩
+
+theorem Command.skip_left (c: Command): (Command.seq .skip c).equiv c := by
+  unfold Command.equiv
+  intro s₁ s₂
+  apply Iff.intro
+  · intro h
+    cases h with
+      | seq c₁ c₂ s₁ s₂ s₃ h₁ h₂ =>
+        cases h₁ with
+          | skip => exact h₂
+  · intro h
+    cases h
+    <;> try (apply CommandEval.seq
+             · apply CommandEval.skip
+             . constructor
+               repeat assumption)
+    case ifFalse =>
+      apply CommandEval.seq
+      · apply CommandEval.skip
+      . apply CommandEval.ifFalse
+        repeat assumption
+    case whileFalse =>
+      apply CommandEval.seq
+      · apply CommandEval.skip
+      · apply CommandEval.whileFalse
+        repeat assumption
+
+
+example (c: Command): (Command.seq c .skip).equiv c :=
+  fun s₁ s₂ =>
+    have mp: CommandEval (Command.seq c .skip) s₁ s₂ → CommandEval c s₁ s₂
+      | .seq c .skip s₁ s _ h₁ (.skip _) => h₁
+    have mpr: CommandEval c s₁ s₂ → CommandEval (Command.seq c .skip) s₁ s₂
+      | .skip _                        => .seq _ _ _ _ _ (.skip _) (.skip _)
+      | .assign _ _ _ _ h              => .seq _ _ _ _ _ (.assign _ _ _ _ h) (.skip _)
+      | .seq _ _ _ s₂ _ h₁ h₂          => .seq _ _ _ _ _ (.seq _ _ _ s₂ _ h₁ h₂) (.skip _)
+      | .ifTrue _ _ _ _ _ h₁ h₂        => .seq _ _ _ _ _ (.ifTrue _ _ _ _ _ h₁ h₂) (.skip _)
+      | .ifFalse _ _ _ _ _ h₁ h₂       => .seq _ _ _ _ _ (.ifFalse _ _ _ _ _ h₁ h₂) (.skip _)
+      | .whileTrue _ s₂ _ _ _ h₁ h₂ h₃ => .seq _ _ _ _ _ (.whileTrue _ s₂ _ _ _ h₁ h₂ h₃) (.skip _)
+      | .whileFalse _ _ _ h₁           => .seq _ _ _ _ _ (.whileFalse _ _ _ h₁) (.skip _)
+    ⟨mp, mpr⟩
+
+theorem Command.skip_right (c: Command): (Command.seq c .skip).equiv c := by
+  unfold Command.equiv
+  intro s₁ s₂
+  apply Iff.intro
+  · intro h
+    cases h with
+      | seq c₁ c₂ s₁ s₂ s₃ h₁ h₂ =>
+        cases h₂ with
+          | skip => exact h₁
+  · intro h
+    cases h
+    <;> try (apply CommandEval.seq
+             . constructor
+               repeat assumption
+             · apply CommandEval.skip)
+    case ifFalse =>
+      apply CommandEval.seq
+      . apply CommandEval.ifFalse
+        repeat assumption
+      · apply CommandEval.skip
+    case whileFalse =>
+      apply CommandEval.seq
+      · apply CommandEval.whileFalse
+        repeat assumption
+      · apply CommandEval.skip
+
+example (t f: Command): (Command.if .true t f).equiv t :=
+  fun s₁ s₂ =>
+    have mp: CommandEval (.if .true t f) s₁ s₂ → CommandEval t s₁ s₂
+      | .ifTrue _ _ _ _ _ _ h₂ => h₂
+      | .ifFalse _ _ _ _ _ _ _ => by contradiction -- TODO: Remove the tactic block
+    have mpr: CommandEval t s₁ s₂ → CommandEval (.if .true t f) s₁ s₂
+      | .skip _                        => .ifTrue _ _ _ _ _ rfl (.skip _)
+      | .assign _ _ _ _ h              => .ifTrue _ _ _ _ _ rfl (.assign _ _ _ _ h)
+      | .seq _ _ _ s _ h₁ h₂           => .ifTrue _ _ _ _ _ rfl (.seq _ _ _ s _ h₁ h₂)
+      | .ifTrue _ _ _ _ _ h₁ h₂        => .ifTrue _ _ _ _ _ rfl (.ifTrue _ _ _ _ _ h₁ h₂)
+      | .ifFalse _ _ _ _ _ h₁ h₂       => .ifTrue _ _ _ _ _ rfl (.ifFalse _ _ _ _ _ h₁ h₂)
+      | .whileTrue _ s₂ _ _ _ h₁ h₂ h₃ => .ifTrue _ _ _ _ _ rfl (.whileTrue _ s₂ _ _ _ h₁ h₂ h₃)
+      | .whileFalse _ _ _ h            => .ifTrue _ _ _ _ _ rfl (.whileFalse _ _ _ h)
+    ⟨mp, mpr⟩
+
+theorem Command.if_true_simple (t f: Command): (Command.if .true t f).equiv t := by
+  unfold Command.equiv
+  intro s₁ s₂
+  apply Iff.intro
+  · intro h
+    cases h with
+      | ifTrue _ _ _ _ _ _ h₂ => exact h₂
+      | ifFalse => contradiction
+  · intro h
+    cases h
+    <;> try (apply CommandEval.ifTrue
+             · unfold Logic.eval
+               rfl
+             · constructor
+               repeat assumption)
+
+    case ifFalse c t f h₁ h₂ =>
+      apply CommandEval.ifTrue
+      · unfold Logic.eval
+        rfl
+      . constructor
+        · sorry
+        · sorry
+    case whileFalse c b h₁ =>
+      apply CommandEval.ifTrue
+      · unfold Logic.eval
+        rfl
+      . constructor
+        · sorry
+        · sorry
+        · sorry
+        · sorry
+
+example (b: Logic) (c₁ c₂: Command) (h₁: b.equiv .true): (Command.if b c₁ c₂).equiv c₁ := by sorry
+theorem Command.if_true (b: Logic) (c₁ c₂: Command) (h₁: b.equiv .true): (Command.if b c₁ c₂).equiv c₁ := by sorry
+
+example (b: Logic) (c₁ c₂: Command) (h₁: b.equiv .false): (Command.if b c₁ c₂).equiv c₂ := by sorry
+theorem Command.if_false (b: Logic) (c₁ c₂: Command) (h₁: b.equiv .false): (Command.if b c₁ c₂).equiv c₂ := by sorry
+
+example (b: Logic) (c₁ c₂: Command): (Command.if b c₁ c₂).equiv (Command.if (.not b) c₂ c₁) := sorry
+theorem Command.if_swap (b: Logic) (c₁ c₂: Command): (Command.if b c₁ c₂).equiv (Command.if (.not b) c₂ c₁) := by sorry
+
+example (c: Logic) (b: Command) (h₁: c.equiv .false): (Command.while c b).equiv Command.skip :=
+  sorry
+  where
+    while_false_nonterm: Nat := sorry
+theorem Command.while_false (c: Logic) (b: Command) (h₁: c.equiv .false): (Command.while c b).equiv Command.skip := by
+  sorry
+  where
+    while_false_nonterm: Nat := sorry
+
+example (c: Logic) (b: Command) (h₁: c.equiv .true): (Command.while c b).equiv (Command.while .true Command.skip) :=
+  sorry
+  where
+    while_true_nonterm: Nat := sorry
+theorem Command.while_true (c: Logic) (b: Command) (h₁: c.equiv .true): (Command.while c b).equiv (Command.while .true Command.skip) := by
+  sorry
+  where
+    while_true_nonterm: Nat := sorry
+
+example (c: Logic) (b: Command): (Command.while c b).equiv (Command.if c (Command.seq b (Command.while c b)) .skip) := sorry
+theorem Command.loop_unrolling (c: Logic) (b: Command): (Command.while c b).equiv (Command.if c (Command.seq b (Command.while c b)) .skip) := by sorry
+
+example (c₁ c₂ c₂: Command): (Command.seq (Command.seq c₁ c₂) c₃).equiv (Command.seq c₁ (Command.seq c₂ c₃)) := sorry
+theorem Command.seq_assoc (c₁ c₂ c₂: Command): (Command.seq (Command.seq c₁ c₂) c₃).equiv (Command.seq c₁ (Command.seq c₂ c₃)) := by sorry
+
+example (id: String): (Command.assign "X" "X").equiv Command.skip := sorry
+theorem Command.identity_assignment (id: String): (Command.assign "X" "X").equiv Command.skip := by sorry
+
+example (id: String) (e: Arith) (h₁: (id: Arith).equiv e): Command.skip.equiv (Command.assign id e) := sorry
+theorem Command.assign_arith_equiv (id: String) (e: Arith) (h₁: (id: Arith).equiv e): Command.skip.equiv (Command.assign id e) := by sorry
+
+section
+  private def a: Command :=
+    .while (.gt "X" 0)
+      (.assign "X" ("X" + 1))
+
+  private def b: Command :=
+    .seq
+      (.if (.eq "X" 0)
+        (.seq
+          (.assign "X" ("X" + 1))
+          (.assign "Y" 1))
+        (.assign "Y" 0))
+      (.seq
+        (.assign "X" ("X" - "Y"))
+        (.assign "Y" 0))
+
+  private def c: Command :=
+    .skip
+
+  private def d: Command :=
+    .while (.neq "X" 0)
+      (.assign "X" ("X" * "Y" + 1))
+
+  private def e: Command :=
+    .assign "Y" 0
+
+  private def f: Command :=
+    .seq
+      (.assign "Y" ("X" + 1))
+      (.while (.neq "X" "Y")
+        (.assign "Y" ("X" + 1)))
+
+  private def g: Command :=
+    .while .true .skip
+
+  private def h: Command :=
+    .while (.neq "X" "X")
+      (.assign "X" ("X" + 1))
+
+  private def i: Command :=
+    .while (.neq "X" "Y")
+      (.assign "X" ("Y" + 1))
+
+  private def equiv_classes: List (List Command) := []
+end
+
+/-
+## Properties of Behavioral Equivalence
+-/
