TacticsCheatSheet.md
@@ -12,7 +12,7 @@ Tactics
 | `intros` | `intro` | Lean4 also supports pattern matching |
 | `reflexivity` | `rfl` | |
 | `apply` | `apply` | |
-| `apply ... in` | ??? | |
+| `apply ... in` | ??? | How do I do an `apply` to a hypothesis in the context? |
 | `apply ... with` | `apply` | Supports explicit positional args (`apply foo 1 2 3`) or named args (`apply foo (x := 1) (z := 3)`) |
 | `simpl` | `simp` | Also has variants `simp [... theorems ...]`, `simp only [... theorems ...]`, `simp_all`, and other more specialized varieties.  Theorems can be added to the simplifier using the `@[simp]`, `@[local simp]` (restricted to the current file), and `@[scoped simp]` (restricted to the current scope and all sub-scopes) annotations.  Any theorem added to the simplifier should "make progress" when read left to right.  So `x + 0 = x` is a good candidate, but `x + y = y + x` is not. |
 | `simpl in h` | `simp at h` | |
@@ -30,7 +30,7 @@ Tactics
 | `assert (H: e)` or `assert (e) as H` | `have h: ... := ...` | `have` is very similar to a local `let` binding.  The name is optional, and defaults to the name `this`. |
 | `generalize dependent` | `generalize` or `revert` | ???.  Not sure which... |
 | `f_equal` | `funext` | ???.  Maybe? |
-| | `contradiction` | Handles a lot of cases, some of which are covered by the Coq `injection` and `discriminate` tactics. |
+| | `contradiction` | Handles a lot of cases, some of which are covered by the Coq `injection` and `discriminate` tactics (I think...). |
 | `left`, `right` | ??? | |
 | `inversion` | ??? | Really want to figure this one out |
 | `lia` | `linarith` | Requires `import Mathlib.tactic.linarith` |
